Hack to support events and random execution path in interpreter.

interpreter.v
@@ -3,33 +3,42 @@
 Require Import String hashset streams.
 Require Export executable frontend natural_type_environment two_complement.
 Local Open Scope string_scope.
+Local Open Scope list_scope.
+
+Record istate (Ti E : Set) := IState {
+  events_new : list E; (**i the events generated in the last step *)
+  events_all : list E; (**i all previously generated events,
+    including those in the last step *)
+  sem_state : state Ti
+}.
+Arguments IState {_ _} _ _ _.
+Instance istate_dec {Ti E : Set}
+  `{∀ k1 k2 : Ti, Decision (k1 = k2), ∀ ε1 ε2 : E, Decision (ε1 = ε2)}
+  (iS1 iS2 : istate Ti E) : Decision (iS1 = iS2).
+Proof. solve_decision. Defined.
 
 Section interpreter.
 Context (be : bool) (Csz : nat).
 Notation Ti := (irank be Csz).
 Context (ptr_size : type Ti → nat) (align_base : base_type Ti → nat).
-Context  (hash : state Ti → Z).
+Context {E : Set} `{∀ ε1 ε2 : E, Decision (ε1 = ε2)}.
+Context (e : state Ti → list E).
 
 Let interpreter_env := (natural_env ptr_size align_base).
 Existing Instance interpreter_env.
 
 Definition cstep_exec' (Γ : env Ti) (δ : funenv Ti)
-    (S : state Ti) : listset (state Ti) * listset (state Ti) :=
-  let Ss := cstep_exec Γ δ S in
-  if decide (listset_car Ss = []) then ({[ S ]}, ∅) else (∅, Ss).
-Definition csteps_exec (Γ : env Ti) (δ : funenv Ti) :
-    listset (state Ti) → stream (listset (state Ti) * listset (state Ti)) :=
-  cofix go Ss :=
-  let Sss := cstep_exec' Γ δ <$> Ss in
-  let nfs := listset_normalize hash (Sss ≫= fst) in
-  let reds := listset_normalize hash (Sss ≫= snd) in
-  (nfs,reds) :.: go reds.
-Definition interpreter (Θ : list (N * decl Ti))
-    (f : funname) (ces : list (cexpr Ti)) :
-    string + stream (listset (state Ti) * listset (state Ti)) :=
+    (iS : istate Ti E) : listset (istate Ti E) :=
+  let (_,εs,S) := iS in
+  (λ S_new,
+    let εs_new := e S_new in IState εs_new (εs ++ εs_new) S_new
+  ) <$> cstep_exec Γ δ S.
+Definition interpreter_initial
+    (Θ : list (N * decl Ti)) (f : funname) (ces : list (cexpr Ti)) :
+    string + (env Ti * funenv Ti * istate Ti E) :=
   '(Γn,Γ,Γf,δ,m,xs) ← to_envs Θ;
   '(σs,_) ← error_of_option (Γf !! f)
-    "interpreter called for undeclared function";
+    "interpreter called with undeclared function";
   eσlrs ← mapM (to_expr Γn Γ Γf m xs) ces;
   let σes := zip_with to_R_NULL σs eσlrs in 
   guard (Forall2 (cast_typed Γ) (snd <$> σes) σs)
@@ -37,5 +46,42 @@ Definition interpreter (Θ : list (N * decl Ti))
   let es := (cast{σs}* (fst <$> σes))%E in
   vs ← error_of_option (mapM (λ e, ⟦ e ⟧ Γ ∅ [] m ≫= maybe_inr) es)
     "interpreter called with non-constant expressions";
-  inr (csteps_exec Γ δ {[ initial_state m f vs ]}).
+  inr (Γ, δ, IState [] [] (initial_state m f vs)).
+
+Context (hash : istate Ti E → Z).
+Definition cstep_exec_all (Γ : env Ti) (δ : funenv Ti) (iS : istate Ti E) :
+    listset (istate Ti E) * listset (istate Ti E) :=
+  let nexts := cstep_exec' Γ δ iS in
+  if decide (nexts ≡ ∅) then (∅, {[ iS ]}) else (nexts, ∅).
+Definition csteps_exec_all (Γ : env Ti) (δ : funenv Ti) :
+    listset (istate Ti E) →
+    stream (listset (istate Ti E) * listset (istate Ti E)) :=
+  cofix go iSs :=
+  let nexts := cstep_exec_all Γ δ <$> iSs in
+  let nfs := listset_normalize hash (nexts ≫= fst) in
+  let reds := listset_normalize hash (nexts ≫= snd) in
+  (nfs,reds) :.: go reds.
+Definition interpreter_all
+    (Θ : list (N * decl Ti)) (f : funname) (ces : list (cexpr Ti)) :
+    string +
+    stream (listset (istate Ti E) * listset (istate Ti E)) :=
+  '(Γ,δ,iS) ← interpreter_initial Θ f ces;
+  inr (csteps_exec_all Γ δ {[ iS ]}).
+
+Context (rand : nat → nat).
+
+Definition csteps_exec_rand (Γ : env Ti) (δ : funenv Ti) :
+    istate Ti E → stream (istate Ti E + istate Ti E) :=
+  cofix go iS :=
+  match listset_car (cstep_exec' Γ δ iS) with
+  | [] => srepeat (inr iS)
+  | (iS' :: _) as iSs =>
+     let next := from_option iS' (iSs !! rand (length iSs)) in
+     inl next :.: go next
+  end.
+Definition interpreter_rand
+    (Θ : list (N * decl Ti)) (f : funname) (ces : list (cexpr Ti)) :
+    string + stream (istate Ti E + istate Ti E) :=
+  '(Γ,δ,iS) ← interpreter_initial Θ f ces;
+  inr (csteps_exec_rand Γ δ iS).
 End interpreter.
